src/kernel_syntax.mli
@@ -2,4 +2,6 @@
     syntax extracted from Coq. *)
 
 val to_kernel : Syntax.formula -> Zfcert_kernel.formula
+val to_kernel_term : Syntax.term -> Zfcert_kernel.named_term
 val of_kernel : Zfcert_kernel.formula -> Syntax.formula
+val of_kernel_term : Zfcert_kernel.named_term -> Syntax.term
