src/syntax.mli
@@ -1,8 +1,8 @@
 type formula =
   | Bottom
   | Named of string * string list
-  | Eq of string * string
-  | Mem of string * string
+  | Eq of term * term
+  | Mem of term * term
   | Not of formula
   | And of formula * formula
   | Or of formula * formula
@@ -11,12 +11,17 @@ type formula =
   | Forall of string * formula
   | Exists of string * formula
 
+and term =
+  | Name of string
+  | App of string * term list
+
 module StringSet : Set.S with type elt = string
 
 val formula_to_string : ?outer:int -> formula -> string
+val term_to_string : term -> string
 val free_vars : formula -> StringSet.t
 val all_vars : formula -> StringSet.t
 val fresh_name : string -> StringSet.t -> string
 val rename_bound : string -> string -> formula -> formula
-val subst : string -> string -> formula -> formula
+val subst : string -> term -> formula -> formula
 val alpha_equal : formula -> formula -> bool
